working on typing judgement

FiatFormal/Language/TyJudge.v
@@ -1,94 +1,121 @@
 
 Require Export FiatFormal.Language.Exp.
 
-
 (* Type Judgement assigns a type to an expression. *)
-Inductive TYPEProg : defs -> delt -> tyenv -> prog -> ty -> Prop :=
-(* Typing an ADT-less program *)
-| TYExp
-  : forall x ds dlt te t1,
-    TYPEX ds dlt te x t1
-    -> TYPEProg ds dlt te (PExp x) t1
-(* Typing program with ADTs *)
-| TYAdtProg
-  : forall p ds dlt te t1,
-    (* type adt under the current environment *)
-
-
-    -> TYPEProg ds dlt te (PAdt adt p)
-
-
-with TYPEX : defs -> delt -> tyenv -> exp -> ty -> Prop :=
+Inductive TYPE : alg_defs -> adt_defs -> tyenv -> exp -> ty -> Prop :=
  (* Variables *)
  | TYVar
-   :  forall ds te i t
-   ,  get i te = Some t
-   -> TYPE ds te (XVar i) t
+   :  forall alg_ds adt_ds te i t,
+     get i te = Some t
+   -> TYPE alg_ds adt_ds te (XVar i) t
 
  (* Lambda Abstraction *)
  | TYLam
-   :  forall ds te x t1 t2
-   ,  TYPE ds (te :> t1) x            t2
-      -> TYPE ds te         (XLam t1 x) (TFun t1 t2)
+   :  forall alg_ds adt_ds te x t1 t2,
+     TYPE alg_ds adt_ds (te :> t1) x            t2
+     -> TYPE alg_ds adt_ds te         (XLam t1 x) (TFun t1 t2)
 
  | TYFix
-   : forall ds te t1 t2 x1
-   , TYPE ds (te :> (TFun t1 t2) :> t1) x1 t2
+   : forall alg_ds adt_ds te t1 t2 x1,
+     TYPE alg_ds adt_ds (te :> (TFun t1 t2) :> t1) x1 t2
      (* TODO: reconsider after defining step relation for fix *)
-     -> TYPE ds te (XFix t1 t2 x1) (TFun t1 t2)
+     -> TYPE alg_ds adt_ds te (XFix t1 t2 x1) (TFun t1 t2)
 
  (* Applications *)
  | TYApp
-   :  forall ds te x1 x2 t1 t2
-   ,  TYPE ds te x1           (TFun t1 t2)
-   -> TYPE ds te x2           t1
-   -> TYPE ds te (XApp x1 x2) t2
+   :  forall alg_ds adt_ds te x1 x2 t1 t2,
+     TYPE alg_ds adt_ds te x1           (TFun t1 t2)
+   -> TYPE alg_ds adt_ds te x2           t1
+   -> TYPE alg_ds adt_ds te (XApp x1 x2) t2
 
  (* Data Constructors *)
  | TYCon
-   :  forall ds te xs dc dcs tsArgs tc
-   ,  getDataDef dc ds = Some (DefData     dc tsArgs (TCon tc))
-   -> getTypeDef tc ds = Some (DefDataType tc dcs)
+   :  forall alg_ds adt_ds te xs dc dcs tsArgs tc,
+     getDataDef dc alg_ds = Some (DefData     dc tsArgs (TCon tc))
+   -> getTypeDef tc alg_ds = Some (DefDataType tc dcs)
    -> In dc dcs
-   -> Forall2 (TYPE ds te) xs tsArgs
-   -> TYPE ds te (XCon dc xs) (TCon tc)
+   -> Forall2 (TYPE alg_ds adt_ds te) xs tsArgs
+   -> TYPE alg_ds adt_ds te (XCon dc xs) (TCon tc)
 
  (* Match Expressions *)
  | TYMatch
-   :  forall ds te xObj tcPat tResult alts dcs
+   :  forall alg_ds adt_ds te xObj tcPat tResult alts dcs,
 
       (* check types of expression and alternatives *)
-   ,  TYPE ds te xObj (TCon tcPat)
-   -> Forall (fun alt => TYPEA ds te alt (TCon tcPat) tResult) alts
+     TYPE alg_ds adt_ds te xObj (TCon tcPat)
+   -> Forall (fun alt => TYPEA alg_ds adt_ds te alt (TCon tcPat) tResult) alts
 
       (* there must be at least one alternative *)
    -> length alts > 0
 
       (* all data cons must have a corresponding alternative *)
-   -> getTypeDef tcPat ds = Some (DefDataType tcPat dcs)
+   -> getTypeDef tcPat alg_ds = Some (DefDataType tcPat dcs)
    -> Forall (fun dc => In dc (map dcOfAlt alts)) dcs
 
-   -> TYPE ds te (XMatch xObj alts) tResult
+   -> TYPE alg_ds adt_ds te (XMatch xObj alts) tResult
 
  | TYChoice
-   : forall t1 t2 xs P,
-     TYPEP ds te P t2
-     -> TYPE ds te (XChoice t1 xs P) t1
+   : forall alg_ds adt_ds t1 t2 xs te P,
+     TYPEP alg_ds adt_ds te P t2
+     -> TYPE alg_ds adt_ds te (XChoice t1 xs P) t1
 
-with TYPEP : defs -> tyenv -> fpred -> ty -> Prop :=
-     | TYPred : forall ds te pc t1,
-         TYPEP ds te (FPred pc) (TPred pc)
+ | TYCall
+   : forall alg_ds adt_ds ac n te s xs,
+     (* check that all adts are well typed *)
+     WELL_TYPED_ADTS alg_ds adt_ds
+     -> getADTSig ac n adt_ds = Some s
+     -> Forall2 (TYPE alg_ds adt_ds te) xs (buildMethodTyEnv (TAdt ac) s)
+     -> TYPE alg_ds adt_ds te (XCall ac n xs) s.(cod)
 
-with TYPEA : defs -> tyenv -> alt -> ty -> ty -> Prop :=
- (* Match Alternatives *)
- | TYAlt
-   :  forall ds te x1 t1 dc tsArgs tResult
-   ,  getDataDef dc ds = Some (DefData dc tsArgs tResult)
-   -> TYPE  ds (te >< tsArgs) x1 t1
-   -> TYPEA ds te (AAlt dc tsArgs x1) tResult t1.
+with WELL_TYPED_ADTS : alg_defs -> adt_defs -> Prop :=
+     (* TODO: consider whether or not a tyenv needed *)
+     | TYADTS : forall alg_ds adt_ds,
+         Forall (WELL_TYPED_ADT alg_ds adt_ds) (getADTCons adt_ds)
+         -> WELL_TYPED_ADTS alg_ds adt_ds
+
+with WELL_TYPED_ADT : alg_defs -> adt_defs -> adtcon -> Prop :=
+     | TYADT : forall alg_ds adt_ds ac adt_d r ss xs,
+         getADTDef ac adt_ds = Some adt_d
+         -> getRep adt_d = r
+         -> getSigs adt_d = ss
+         -> getBodies adt_d = xs
+         (* ensure that cod = (FiatProdType)? *)
+         -> Forall3 (TYPE alg_ds adt_ds) (map (buildMethodTyEnv r) ss) xs (map cod ss) (* TODO: cod needs to reference Rep, not opaque type variable *)
+         -> WELL_TYPED_ADT alg_ds adt_ds ac
+
+with TYPEP : alg_defs -> adt_defs -> tyenv -> fpred -> ty -> Prop :=
+     (* placeholder for predicate typing -- this is old *)
+     | TYPred : forall alg_ds adt_ds te pc,
+         TYPEP alg_ds adt_ds te (FPred pc) (TPred pc)
+
+with TYPEA : alg_defs -> adt_defs -> tyenv -> alt -> ty -> ty -> Prop :=
+     (* Match Alternatives *)
+     | TYAlt
+       :  forall alg_ds adt_ds te x1 t1 dc tsArgs tResult,
+         getDataDef dc alg_ds = Some (DefData dc tsArgs tResult)
+         -> TYPE  alg_ds adt_ds (te >< tsArgs) x1 t1
+         -> TYPEA alg_ds adt_ds te (AAlt dc tsArgs x1) tResult t1.
 
 Hint Constructors TYPE.
 Hint Constructors TYPEA.
+Hint Constructors TYPEP.
+Hint Constructors WELL_TYPED_ADTS.
+Hint Constructors WELL_TYPED_ADT.
+
+(* Inductive wellTypedMethod : *)
+
+
+(* Inductive wfDef : def -> Prop := *)
+(* | WF_DTYPE : forall tc dcs, wfDef (DefDataType tc dcs) *)
+(* | WF_DATA  : forall dc ts tResult, wfDef (DefDataType dc ts tResult) *)
+(* | WF_ADT   : forall ac r sigs xs ds te, *)
+(*     let sigs' := map (replace_TAdt_with_Rep r ac) sigs *)
+(*     in *)
+(*     Forall2 (TYPE ds (te >< sigs')) xs (map get_last sigs') *)
+
+(*             Inductive wfDefs : defs -> Prop := *)
+(* | WFD_NIL  : wfDefs nil *)
+(* | WFD_CONS : forall d ds, wfDef d -> wfDefs ds -> wfDefs (ds :> d). *)
 
 
 (* Invert all hypothesis that are compound typing statements. *)
@@ -111,9 +138,9 @@ Ltac inverts_type :=
    If we know the type of a value,
    then we know the form of that value. *)
 Lemma value_lam
- :  forall x ds te t1 t2
+ :  forall x alg_ds adt_ds te t1 t2
  ,  value x
- -> TYPE ds te x (TFun t1 t2)
+ -> TYPE alg_ds adt_ds te x (TFun t1 t2)
  -> (exists t x', x = XLam t x') \/ (exists t1 t2 x', x = XFix t1 t2 x'). (* TODO *)
 Proof.
 (*  intros. destruct x; burn. *)
@@ -125,9 +152,9 @@ Hint Resolve value_lam.
 (********************************************************************)
 (* A well typed expression is well formed *)
 Theorem type_wfX
- :  forall ds te x t
- ,  TYPE ds te x t
- -> wfX te x.
+  :  forall alg_ds adt_ds te x t,
+    TYPE alg_ds adt_ds te x t
+    -> wfX te x.
 Proof.
 (*  intros. gen ds te t. *)
 (*  induction x using exp_mutind with  *)
@@ -155,9 +182,9 @@ Hint Resolve type_wfX.
    lift existing references to types higher in the stack across
    the new one. *)
 Lemma type_tyenv_insert
- :  forall ds te ix x t1 t2
- ,  TYPE ds te x t1
- -> TYPE ds (insert ix t2 te) (liftX 1 ix x) t1.
+ :  forall alg_ds adt_ds te ix x t1 t2
+ ,  TYPE alg_ds adt_ds te x t1
+ -> TYPE alg_ds adt_ds (insert ix t2 te) (liftX 1 ix x) t1.
 Proof.
 (*  intros. gen ix ds te t1. *)
 (*  induction x using exp_mutind with  *)
@@ -206,9 +233,9 @@ Admitted.
 (* We can push a new type onto the environment stack provided
    we lift references to existing types across the new one. *)
 Lemma type_tyenv_weaken1
- :  forall ds te x t1 t2
- ,  TYPE ds te x t1
- -> TYPE ds (te :> t2) (liftX 1 0 x) t1.
+ :  forall alg_ds adt_ds te x t1 t2
+ ,  TYPE alg_ds adt_ds te x t1
+ -> TYPE alg_ds adt_ds (te :> t2) (liftX 1 0 x) t1.
 Proof.
 (*  intros. *)
 (*  rrwrite (te :> t2 = insert 0 t2 te). *)
@@ -219,9 +246,9 @@ Admitted.
 (* We can push several new types onto the environment stack provided
    we lift referenes to existing types across the new one. *)
 Lemma type_tyenv_weaken_append
- :  forall ds te te' x t1
- ,  TYPE ds te x t1
- -> TYPE ds (te >< te') (liftX (length te') 0 x) t1.
+ :  forall alg_ds adt_ds te te' x t1
+ ,  TYPE alg_ds adt_ds te x t1
+ -> TYPE alg_ds adt_ds (te >< te') (liftX (length te') 0 x) t1.
 Proof.
 (*  intros. *)
 (*  induction te'; simpl. *)
