FiatFormal/Language/Alg.v
@@ -1,0 +1,78 @@
+
+Require Export FiatFormal.Language.Ty.
+
+
+(* Definitions.
+   Carries meta information about type and data constructors *)
+Inductive alg_def : Type :=
+ (* Definition of a data type constructor *)
+ | DefDataType
+   :  tycon        (* Name of data type constructor *)
+   -> list datacon (* Data constructors that build this type *)
+   -> alg_def
+
+ (* Definition of a data constructor *)
+ | DefData
+   :  datacon      (* Name of data constructor *)
+   -> list ty      (* Types of arguments *)
+   -> ty           (* Type  of constructed data *)
+   -> alg_def.
+Hint Constructors alg_def.
+
+
+(* Definition environment *)
+Definition alg_defs  := list alg_def.
+
+
+(* Functions for looking up definitions by (tycon, datacon) *)
+
+(* Lookup the definition of a given type constructor *)
+Fixpoint getTypeDef (tc: tycon) (ds: alg_defs) : option alg_def :=
+ match ds with
+ | ds' :> DefDataType tc' _ as d
+ => if tycon_beq tc tc'
+     then  Some d
+     else  getTypeDef tc ds'
+
+ | ds' :> _ => getTypeDef tc ds'
+ | Empty    => None
+ end.
+(* Lookup the definition of a given data constructor *)
+Fixpoint getDataDef (dc: datacon) (ds: alg_defs) : option alg_def :=
+ match ds with
+ | ds' :> DefData dc' _ _ as d
+ => if datacon_beq dc dc'
+     then  Some d
+     else  getDataDef dc ds'
+
+ | ds' :> _ => getDataDef dc ds'
+ | Empty    => None
+ end.
+
+
+(* Some proofs about equality between these "name" constructors *)
+Lemma datacon_beq_eq
+ :  forall dc dc'
+ ,  true = datacon_beq dc dc'
+ -> dc = dc'.
+Proof.
+ intros.
+ destruct dc.
+ destruct dc'.
+ simpl in H.
+ apply beq_nat_eq in H.
+ auto.
+Qed.
+Lemma datacon_beq_false
+ :  forall dc
+ ,  false = datacon_beq dc dc
+ -> False.
+Proof.
+ intro.
+ destruct dc.
+ simpl.
+ intros.
+  induction n.
+  simpl in H. inversion H.
+  simpl in H. auto.
+Qed.
